finished!

src/week_2/kb_solutions/Part_B_subgroups_solutions.lean
@@ -4,7 +4,9 @@ import week_2.kb_solutions.Part_A_groups_solutions
 
 ## Subgroups
 
-Lean has subgroups already, so we'll call ours subgroup2.
+We define the structure `subgroup G`, whose terms are subgroups of `G`.
+A subgroup of `G` is implemented as a subset of `G` closed under
+`1`, `*` and `⁻¹`.
 
 -/
 
@@ -22,16 +24,21 @@ structure subgroup (G : Type) [group G] :=
 
 At this point, here's what we have.
 
-A term `H` of type `subgroup2 G`, written `H : subgroup2 G`, is a
-quadruple `H.carrier` (a subset of `G`), `H.one_mem'` (a proof
-that `1 ∈ H.carrier`), `H.mul_mem'` (a proof that if `x` and `y` are in
-`H.carrier` then so is `x*y`) and `H.inv_mem'` (saying `H` is closed under
-inverses). Note here that the _type_ of `x` and `y` is still `G`, 
+A term `H` of type `subgroup G`, written `H : subgroup G`, is a
+*quadruple*. To give a term `H : subgroup G` is to give the following four things:
+1) `H.carrier` (a subset of `G`),
+2) `H.one_mem'` (a proof that `1 ∈ H.carrier`),
+3) `H.mul_mem'` (a proof that `H` is closed under multiplication)
+4) `H.inv_mem'` (a proof that `H` is closed under inverses).
+
+Note in particular that Lean, being super-pedantic, *distinguishes* between
+the subgroup `H` and the subset `H.carrier`. One is a subgroup, one is
+a subset. When we get going we will start by setting up some infrastructure
+so that this difference will be hard to notice.
+
+Note also that if `x` is in the subgroup `H` of `H` then the _type_ of `x` is still `G`,
 and `x ∈ carrier` is a Proposition. Note also that `x : carrier` doesn't
 make sense (`carrier` is a term, not a type, rather counterintuitively).
-
-This kind of stinks. I don't want to write `H.carrier` everywhere.
-I want to write `H`. Let's start by sorting this out.
 
 -/
 
@@ -40,37 +47,68 @@ namespace subgroup
 open xena.group
 
 -- let G be a group and let H and K be subgroups
-variables {G : Type} [group G] (H K : subgroup G)
+variables {G : Type} [group G] (H J K : subgroup G)
 
--- If `x : G` and `H : subgroup2 G` then let's define `x ∈ H` to mean
--- `x ∈ H.carrier`
+/-
+This `h ∈ H.carrier` notation kind of stinks. I don't want to write `H.carrier`
+everywhere, because I want to be able to identify the subgroup `H` with
+its underlying subset `H.carrier`. Note that these things are not _equal_,
+firstly because `H` contains the proof that `H.carrier` is a subgroup, and
+secondly because these terms have different types! `H` has type `subgroup G`
+and `H.carrier` has type `set G`. Let's start by sorting this out.
+-/
+
+-- If `x : G` and `H : subgroup G` then let's define the notation
+-- `x ∈ H` to mean `x ∈ H.carrier`
 instance : has_mem G (subgroup G) := ⟨λ m H, m ∈ H.carrier⟩
 
--- Now let's define theorems without the `'`s in, which use this
--- more normal notation
+-- Let's also define a "coercion", a.k.a. an "invisible map"
+-- from subgroups of `G` to subsets of `G`, sending `H` to `H.carrier`. 
+-- The map is not completely invisible -- it's a little ↑. So
+-- if you see `↑H` in the future, it means the subset `H.carrier` by definition.
+instance : has_coe (subgroup G) (set G) := ⟨λ H, H.carrier⟩
 
-/-- A subgroup2 contains the group's 1. -/
+-- `λ` is just computer science notation for ↦ (mapsto); so
+-- `λ H, H.carrier` is the function `H ↦ H.carrier`.
+
+-- Let's check we have this working, and also tell the simplifier that we
+-- would rather talk about `g ∈ H` than any other way of saying it.
+
+/-- `g` is in the underlying subset of `H` iff `g ∈ H`. -/
+@[simp] lemma mem_carrier {g : G} : g ∈ H.carrier ↔ g ∈ H :=
+begin
+  -- true by definition
+  refl
+end
+
+/-- `g` is in `H` considered as a subset of `G`, iff `g` is in `H` considered
+as subgroup of `G`. -/
+@[simp] lemma mem_coe {g : G} : g ∈ (↑H : set G) ↔ g ∈ H :=
+begin
+  -- true by definition
+  refl
+end
+
+-- Now let's define theorems without the `'`s in, which use this
+-- more natural notation
+
+/-- A subgroup contains the group's 1. -/
 theorem one_mem : (1 : G) ∈ H :=
 begin
   apply H.one_mem',
 end
 
-/-- A subgroup2 is closed under multiplication. -/
+/-- A subgroup is closed under multiplication. -/
 theorem mul_mem {x y : G} : x ∈ H → y ∈ H → x * y ∈ H :=
 begin
   apply H.mul_mem',
 end
 
-/-- A subgroup2 is closed under inverse -/
+/-- A subgroup is closed under inverse -/
 theorem inv_mem {x : G} : x ∈ H → x⁻¹ ∈ H :=
 begin
   apply H.inv_mem',
 end
-
--- let's tell the simplifier that we would rather talk about `g ∈ H`
--- than `g ∈ H.carrier`
-
-@[simp] lemma mem_coe {g : G} : g ∈ H.carrier ↔ g ∈ H := iff.rfl
 
 /-
 
@@ -81,12 +119,20 @@ Say `H : subgroup G`. Then:
 `H.mul_mem {x y : G} : x ∈ H → y ∈ H → x * y ∈ H`
 `H.inv_mem {x : G} : x ∈ H → x⁻¹ ∈ H`
 
+These now look like the way a mathematician would write things.
+
+Now let's start to prove basic theorems about subgroups (or, as a the computer
+scientists would say, make a basic _interface_ or _API_ for subgroups),
+using this sensible notation.
+
+Here's an example; let's prove `x ∈ H ↔ x⁻¹ ∈ H`. Let's put the more
+complicated expression on the left hand side of the `↔` though, because then
+we can make it a `simp` lemma.
 -/
 
--- now we can prove basic theorems about subgroups using this sensible notation
 -- Remember that `xena.group.inv_inv x` is the statement that `x⁻¹⁻¹ = x`
 
-@[simp] theorem inv_mem_iff {x :G} : x⁻¹ ∈ H ↔ x ∈ H := 
+@[simp] theorem inv_mem_iff {x : G} : x⁻¹ ∈ H ↔ x ∈ H := 
 begin
   split,
   { intro h,
@@ -96,27 +142,40 @@ begin
   { apply H.inv_mem },
 end
 
+-- We could prove a bunch more theorems here. Let's just do one more.
+-- Let's show that if x and xy are in H then so is y.
+
+theorem mem_of_mem_mul_mem {x y : G} (hx : x ∈ H) (hxy : x * y ∈ H) : y ∈ H :=
+begin
+  rw ← inv_mem_iff at hx,
+  convert H.mul_mem hx hxy, -- I claim that this proof that x⁻¹ * (x * y) ∈ H is what we want
+  -- so now it just remains to prove x⁻¹ * (x * y) = y, which we can do because of Knuth-Bendix
+  simp,
+end
+
 /-
 Subgroups are extensional objects (like most things in mathematics):
 two subgroups are equal if they have the same underlying subset,
 and also if they have the same underlying elements.
-Let's prove variants of this triviality now.
+Let's prove variants of this triviality now. The first one is rather
+un-mathematical: it takes a subgroup apart into its pieces. I'll see if
+you can do the other two!
 -/
 
 /-- Two subgroups are equal if the underlying subsets are equal. -/
 theorem ext' {H K : subgroup G} (h : H.carrier = K.carrier) : H = K :=
 begin
   -- first take H and K apart
-  cases H,
+  cases H, -- H now broken up into its underlying 3-tuple.
   cases K,
-  -- and now it must be obvious
-  simp * at *,
+  -- and now it must be obvious, so let's see if the simplifier can do it.
+  simp * at *, -- it can!
 end
 
--- here's a variant
+-- here's a variant. You can prove it using `ext'`. 
 
 /-- Two subgroups are equal if and only if the underlying subsets are equal. -/
-protected theorem ext'_iff {H K : subgroup G} :
+theorem ext'_iff {H K : subgroup G} :
   H.carrier = K.carrier ↔ H = K :=
 begin
   split,
@@ -146,33 +205,115 @@ too: if you ever have a goal of proving that two subgroups are equal, you can
 use the `ext` tactic to reduce to showing that they have the same elements.
 -/
 
--- Coersion to group
--- Coercion from subgroup2 to underlying type
-
-instance : has_coe (subgroup G) (set G) := ⟨subgroup.carrier⟩
-
---lemma mem_coe' {g : G} : g ∈ (H : set G) ↔ g ∈ H := iff.rfl
-
-
-
 /-
+
+## The lattice structure on subgroups
+
 Subgroups of a group form what is known as a *lattice*. 
 This is a partially ordered set with a sensible notion of
-max and min. Subgroups even have a good notion of an infinite
-sup and inf.
+max and min. We partially order subgroups by saying `H ≤ K` if
+`H.carrier ⊆ K.carrier`. Subgroups even have a good notion of an infinite
+Sup and Inf (the Inf of a bunch of subgroups is just their intersection;
+their Sup is the subgroup generated by their union).
 
-We will prove this here.
+This combinatorial structure (a partially ordered set with good
+finite and infinite notions of Sup and Inf) is called a "complete lattice",
+and Lean has this structure inbuilt into it. We will construct
+a complete lattice structure on `subgroup G`.
 
 We start by defining a relation ≤ on the type of subgroups of a group.
 We say H ≤ K iff H.carrier ⊆ K.carrier .
 -/
-instance : has_le (subgroup G) := ⟨λ S T, S.carrier ⊆ T.carrier⟩
+
+/-- If `H` and `K` are subgroups of `G`, we write `H ≤ K` to
+  mean `H.carrier ⊆ K.carrier` -/
+instance : has_le (subgroup G) := ⟨λ H K, H.carrier ⊆ K.carrier⟩
+
+-- useful to restate the definition so we can `rw` it
+lemma le_def : H ≤ K ↔ H.carrier ⊆ K.carrier :=
+begin
+  -- true by definition
+  refl
+end
+
+-- another useful variant
+lemma le_iff : H ≤ K ↔ ∀ g, g ∈ H → g ∈ K :=
+begin
+  -- true by definition
+  refl,
+end
 
 
-open set
 
--- The intersect of two subgroup2s is also a subgroup2
+-- Now let's check the axioms for a partial order.
+-- These are not hard, they just reduce immediately to the
+-- fact that ⊆ is a partial order
+@[refl] lemma le_refl : H ≤ H :=
+begin
+  rw le_def,
+  -- Lean knows ⊆ is reflexive so the sneaky `refl` which Lean tries after `rw` 
+  -- has closed the goal!
+end
+
+lemma le_antisymm : H ≤ K → K ≤ H → H = K :=
+begin
+  rw [le_def, le_def, ← ext'_iff],
+  -- now this is antisymmetry of ⊆, which Lean knows
+  exact set.subset.antisymm,
+end
+
+@[trans] lemma le_trans : H ≤ J → J ≤ K → H ≤ K :=
+begin
+  rw [le_def, le_def, le_def],
+  -- now this is transitivity of ⊆, which Lean knows
+  exact set.subset.trans,
+end
+
+-- We've made `subgroup G` into a partial order!
+instance : partial_order (subgroup G) :=
+{ le := (≤),
+  le_refl := le_refl,
+  le_antisymm := le_antisymm,
+  le_trans := le_trans }
+
+/-
+
+
+### intersections
+
+Let's prove that the intersection of two subgroups is a subgroup. In Lean
+this is a definition: given two subgroups, we define a new subgroup whose
+underlying subset is the intersection of the subsets, and then prove
+the axioms.
+-/
+
+/-- The intersection of two subgroups is also a subgroup -/
 def inf (H K : subgroup G) : subgroup G :=
+{ carrier := H.carrier ∩ K.carrier, -- the carrier is the intersection
+  one_mem' := 
+  begin
+    -- recall that x ∈ Y ∩ Z is _by definition_ x ∈ Y ∧ x ∈ Z, so you can `split` this. 
+    split,
+    { exact H.one_mem },
+    { exact K.one_mem },
+  end,
+  mul_mem' := 
+  begin
+    intros x y hx hy,
+    cases hx with hxH hxK,
+    cases hy with hyH hyK,
+    split,
+    { exact H.mul_mem hxH hyH },
+    { exact K.mul_mem hxK hyK },
+  end,
+  inv_mem' :=
+  begin
+    rintro x ⟨hxH, hxK⟩, -- rintro does intro and cases all in one go
+    exact ⟨H.inv_mem hxH, K.inv_mem hxK⟩, -- ⟨⟩ instead of split
+  end }
+
+-- Note that using "term mode" one can really compactify all this.
+def inf_term_mode (H K : subgroup G) : subgroup G :=
 { carrier := H.carrier ∩ K.carrier,
   one_mem' := ⟨H.one_mem, K.one_mem⟩,
   mul_mem' := λ _ _ ⟨hhx, hkx⟩ ⟨hhy, hky⟩, 
@@ -180,97 +321,307 @@ def inf (H K : subgroup G) : subgroup G :=
   inv_mem' := λ x ⟨hhx, hhy⟩,
   ⟨H.inv_mem hhx, K.inv_mem hhy⟩}
 
-lemma inf_def (H K : subgroup G) : (inf H K : set G) = (H : set G) ∩ K := rfl 
+-- Notation for `inf` in computer science circles is ⊓ .
 
+instance : has_inf (subgroup G) := ⟨inf⟩
+
+/-- The underlying set of the inf of two subgroups is just their intersection -/
+lemma inf_def (H K : subgroup G) : (H ⊓ K : set G) = (H : set G) ∩ K :=
+begin
+  -- true by definition
+  refl
+end
+
+/-
+
+## Subgroup generated by a subset.
+
+To do the sup of two subgroups is harder, because we don't just take
+the union, we need to then look at the subgroup generated by this union
+(e.g. the union of the x and y axes in ℝ² is not a subgroup). So we need
+to have a machine to spit out the subgroup of `G` generated by a subset `S : set G`.
+
+There are two completely different ways to do this. The first is a "top-down"
+approach. We could define the subgroup generated by `S` to be the intersection of
+all the subgroups of `G` that contain `S`. The second is a "bottom-up" approach.
+We could define the subgroup generated by `S` "by induction" (or more precisely
+by recursion), saying that `S` is in the subgroup, 1 is in the subgroup,
+the product of two things in the subgroup is in the subgroup, the
+inverse of something in the subgroup is in the subgroup, and that's it.
+Both methods come out rather nicely in Lean. Let's do the first one.
+
+We are going to be using a bunch of theorems about "bounded intersections",
+a.k.a. `set.bInter`. We will soon get tired of writing `set.blah` so let's
+`open set` so that we can skip it. 
+
+-/
+
+open set
+
+/-
+
+Here is the API for `set.bInter` (or `bInter`, as we can now call it):
+
+Notation: `⋂` (type with `\I`)
+
+If `X : set (subgroup G)`, i.e. if `X` is a set of subgroups of `G`, then
+
+`⋂ K ∈ X, (K : set G)` means "take the intersection of the underlying subsets".
+
+-- mem_bInter_iff says you're in the intersection iff you're in
+-- all the things you're intersecting. Very useful for rewriting.
+`mem_bInter_iff : (g ∈ ⋂ (K ∈ S), f K) ↔ (∀ K, K ∈ s → g ∈ f K)`
+
+-- mem_bInter is just the one way implication. Very useful for `apply`ing.
+`mem_bInter : (∀ K, K ∈ s → g ∈ f K) → (g ∈ ⋂ (K ∈ S), f K)`
+
+-/
 /- 
-We will consider the closure of a set as the intersect of all subgroup2s
+We will consider the closure of a set as the intersect of all subgroups
 containing the set
 -/
-instance : has_Inf (subgroup G) :=
-⟨λ s, {
-  carrier := ⋂ t ∈ s, (t : set G),
+
+/-- The Inf of a set of subgroups of G is their intersection. -/
+def Inf (X : set (subgroup G)) : subgroup G :=
+{ carrier := ⋂ K ∈ X, (K : set G), -- carrier is the intersection of the underlying sets
+  one_mem' := begin
+    apply mem_bInter,
+    intros H hH,
+    apply H.one_mem,
+  end,
+  mul_mem' := begin
+    intros x y hx hy,
+    rw mem_bInter_iff at *,
+    intros H hH,
+    apply H.mul_mem,
+    { apply hx,
+      exact hH },
+    { exact hy H hH }  
+  end,
+  inv_mem' := begin
+    intros x hX,
+    rw mem_bInter_iff at *,
+    intros H hH,
+    exact H.inv_mem (hX H hH),
+  end,
+}
+
+-- again note that term mode can do this much more quickly
+def Inf' (X : set (subgroup G)) : subgroup G :=
+{ carrier := ⋂ t ∈ X, (t : set G),
   one_mem' := mem_bInter $ λ i h, i.one_mem,
   mul_mem' := λ x y hx hy, mem_bInter $ λ i h,
     i.mul_mem (by apply mem_bInter_iff.1 hx i h) 
     (by apply mem_bInter_iff.1 hy i h),
   inv_mem' := λ x hx, mem_bInter $ λ i h,
-    i.inv_mem (by apply mem_bInter_iff.1 hx i h) }⟩
+    i.inv_mem (by apply mem_bInter_iff.1 hx i h) }
 
-def closure (S : set G) : subgroup G := Inf {H | S ⊆ H}
+/-- The *closure* of a subset `S` of `G` is the `Inf` of the subgroups of `G`
+  which contain `S`. -/
+def closure (S : set G) : subgroup G := Inf {H : subgroup G | S ⊆ H}
 
+-- we can restate mem_bInter_iff using our new "closure" language:
 lemma mem_closure_iff {S : set G} {x : G} : 
   x ∈ closure S ↔ ∀ H : subgroup G, S ⊆ H → x ∈ H := mem_bInter_iff
 
-/- We will now prove some lemmas that are helpful in proving subgroups 
-form a galois_insertion with the coercion to set
+/- 
+There is an underlying abstraction here, which you may not know about.
+A "closure operator" in mathematics 
+
+https://en.wikipedia.org/wiki/Closure_operator
+
+is something mapping subsets of a set X to subsets of X, and satisfying three
+axioms:
+
+1) `subset_closure : S ⊆ closure S`
+2) `closure_mono : (S ⊆ T) → (closure S ⊆ closure T)`
+3) `closure_closure : closure (closure S) = closure S`
+
+It works for closure in topological spaces, and it works here too.
+It also works for algebraic closures of fields, and there are several
+other places in mathematics where it shows up. This idea, of "abstracting"
+and axiomatising a phenomenon which shows up in more than one place,
+is really key in Lean.
+
+Let's prove these three lemmas in the case where `X = G` and `closure S`
+is the subgroup generated by `S`.
+
+Here are some things you might find helpful.
+
+Remember 
+`mem_coe : g ∈ ↑H ↔ g ∈ H`
+`mem_carrier : g ∈ H.carrier ↔ g ∈ H`
+
+There's 
+`mem_closure_iff : x ∈ closure S ↔ ∀ (H : subgroup G), S ⊆ ↑H → x ∈ H`
+(`closure S` is a subgroup so you might need to use `mem_coe` or `mem_carrier` first)
+
+For subsets there's
+`subset.trans : X ⊆ Y → Y ⊆ Z → X ⊆ Z`
+
+You might find `le_antisymm : H ≤ K → K ≤ H → H = K` from above useful
 -/
 
-lemma le_closure (S : set G) : S ≤ closure S :=
-λ s hs H ⟨y, hy⟩, by rw ←hy; simp; exact λ hS, hS hs
+/-
+Reminder: X ⊆ Y means `∀ g, g ∈ X → g ∈ Y` and it's definitional,
+so you can just start this with `intro g`.
+-/
+lemma subset_closure (S : set G) : S ⊆ closure S :=
+begin
+  intro g,
+  intro hgS,
+  rw [mem_coe, mem_closure_iff],
+  intros H hH,
+  apply hH,
+  assumption
+end
 
-lemma closure_le (S : set G) (H : subgroup G) : closure S ≤ H ↔ S ⊆ H :=
+-- fancy term mode proof
+lemma subset_closure' (S : set G) : S ⊆ closure S :=
+λ s hs H ⟨y, hy⟩, by {rw [←hy, mem_Inter], exact λ hS, hS hs}
+
+-- It's useful to know `subset.trans : X ⊆ Y → Y ⊆ Z → X ⊆ Z`
+lemma closure_mono {S T : set G} (hST : S ⊆ T) : closure S ≤ closure T :=
+begin
+  intros x hx,
+  rw [mem_carrier, mem_closure_iff] at *,
+  intros H hTH,
+  apply hx,
+  exact subset.trans hST hTH,
+end
+
+-- not one of the axioms, but sometimes handy
+lemma closure_le (S : set G) (H : subgroup G) : closure S ≤ H ↔ S ⊆ ↑H :=
 begin
   split,
-    { intro h, refine subset.trans (le_closure _) h },
-    { intros h y,
-      unfold closure, unfold Inf, 
-      rw mem_bInter_iff, intro hy,
-      exact hy H h }
+    { intro hSH,
+      exact subset.trans (subset_closure S) hSH },
+    { intros hSH g hg,
+      rw [mem_carrier, mem_closure_iff] at hg,
+      exact hg _ hSH }
 end
 
-lemma closure_le' (S : set G) (H : subgroup G) : 
-  (closure S : set G) ⊆ H ↔ S ⊆ H := closure_le S H
-
-lemma closure_le'' (S : set G) (H : subgroup G) : 
-  (∀ x, x ∈ closure S → x ∈ H) ↔ (∀ x, x ∈ S → x ∈ H) := closure_le S H
-
-lemma closure_self {H : subgroup G} : closure (H : set G) = H :=
+-- You can start this one by applying `le_antisymm`,
+lemma closure_closure (S : set G) : closure S = closure (closure S) :=
 begin
-  rw ←subgroup.ext'_iff, ext,
-  split; intro hx,
-    { apply subset.trans _ ((closure_le (H : set G) H).2 (subset.refl H)), 
-      exact hx, exact subset.refl _ },
-    { apply subset.trans (le_closure (H : set G)), 
-      intros g hg, assumption, assumption }
+  apply le_antisymm,
+  { apply subset_closure },
+  { rw closure_le,
+    intros x hx,
+    exact hx }, 
 end
 
-lemma closure_induction {p : G → Prop} {x} {k : set G} (h : x ∈ closure k)
-  (Hk : ∀ x ∈ k, p x) (H1 : p 1)
+-- This shows that every subgroup is the closure of something, namely its
+-- underlying subset. 
+lemma closure_self {H : subgroup G} : closure ↑H = H :=
+begin
+  apply le_antisymm,
+  { rw le_iff,
+    intro g,
+    rw mem_closure_iff,
+    intro h,
+    apply h,
+    refl },
+  { exact subset_closure H }
+end
+
+/-
+Recall the second proposed construction of the subgroup closure of a subset `S`;
+it is the smallest subgroup `H` of `G` such that `S ⊆ H` and which contains
+`1` and is closed under `*` and `⁻¹`. This inductive constuction (which we
+did not make) comes with a so-called "recursor": if we have a true/false
+statement `p g` attached to each element `g` of G with the following properties:
+
+1) `p s` is true for all `s ∈ S`,
+2) `p 1` is true,
+3) If `p x` and `p y` then `p (x * y)`,
+4) If `p x` then `p x⁻¹`
+
+Then `p` is true on all of `closure S`.
+
+If we had made an inductive definition of `closure S` then this would have been true
+by definition! We used another definition, so we will have to prove it
+ourselves.
+-/
+
+/-- An induction principle for closures. -/
+lemma closure_induction {p : G → Prop} {S : set G}
+  (HS : ∀ x ∈ S, p x)
+  (H1 : p 1)
   (Hmul : ∀ x y, p x → p y → p (x * y))
-  (Hinv : ∀ x, p x → p x⁻¹) : p x :=
-(@closure_le _ _ _ ⟨p, H1, Hmul, Hinv⟩).2 Hk h
+  (Hinv : ∀ x, p x → p x⁻¹) : 
+  -- conclusion after colon
+  ∀ x, x ∈ closure S → p x :=
+begin
+  -- the subset of G where `p` is true is a subgroup. Let's call it H
+  let H : subgroup G :=
+  { carrier := p, 
+    one_mem' := H1, 
+    mul_mem' := Hmul,
+    inv_mem' := Hinv },
+  -- The goal is just that closure S ≤ H, by definition.
+  change closure S ≤ H,  
+  -- Our hypothesis HS is just that S ⊆ ↑H, by definition
+  change S ⊆ ↑H at HS, 
+  -- So this is just closure_le in disguise
+  rw closure_le,
+  assumption,
+end
+
+-- this is even briefer in term mode:
+lemma closure_induction' {p : G → Prop} {S : set G}
+  (HS : ∀ x ∈ S, p x)
+  (H1 : p 1)
+  (Hmul : ∀ x y, p x → p y → p (x * y))
+  (Hinv : ∀ x, p x → p x⁻¹) : 
+  ∀ x, x ∈ closure S → p x :=
+λ x h, (@closure_le _ _ _ ⟨p, H1, Hmul, Hinv⟩).2 HS h
 
 /-
-Now, by considering the coercion between subgroup2 G → set G, we cheat a bit
-by transfering the partial order on set to the partial order on subgroups.
+Finally we prove that the `closure` and `coe` maps form a `galois_insertion`.
+This is another abstraction, it generalises `galois_connection`, which is
+something that shows up all over the place (algebraic geometry, Galois theory etc).
+See
 
-We do this because galois_insertion requires preorders and partial orders
-extends preoders.
--/
-instance : partial_order (subgroup G) := 
-{.. partial_order.lift (coe : subgroup G → set G) (λ x y, subgroup.ext')}
+https://en.wikipedia.org/wiki/Galois_connection
 
-/-
-Finially we prove that subgroups form a galois_insertion with the coercion 
-to set.
+A partial order can be considered as a category, with Hom(A,B) having
+one element if A ≤ B and no elements otherwise. A Galois connection between
+two partial orders is just a pair of adjoint functors between the categories.
+Adjointness in our case is `S ⊆ ↑H ↔ closure S ≤ H`. 
+
+The reason it's an insertion and not just a connection is that if you start
+with a subgroup, take the underlying subset, and then look at the subgroup
+generated by that set, you get back to where you started. So it's like one
+of the adjoint functors being a forgetful functor.
 -/
+
 def gi : galois_insertion (closure : set G → subgroup G) (coe : subgroup G → set G) :=
 { choice := λ S _, closure S,
-  gc := λ H K,
-    begin
-      split; intro h,
-        { exact subset.trans (le_closure H) h },
-        { exact (closure_le _ _).2 h },
-    end,
-  le_l_u := λ H, le_closure (H : set G),
+  gc := closure_le,
+  le_l_u := λ H, subset_closure (H : set G),
   choice_eq := λ _ _, rfl }
 
 /-
-With that it follows that subgroup2s form a complete lattice!
+
+One use of this abstraction is that now we can pull back the complete
+lattice structure on `set G` to get a complete lattice structure on `subgroup G`. 
 -/
+
 instance : complete_lattice (subgroup G) :=
 {.. galois_insertion.lift_complete_lattice gi}
 
+/-
+
+We just proved loads of lemmas about Infs and Sups of subgroups automatically,
+and have access to a ton more because the `complete_lattice` structure in
+Lean has a big API. See for example
+
+https://leanprover-community.github.io/mathlib_docs/order/complete_lattice.html#complete_lattice
+
+All those theorems are now true for subgroups. None are particularly hard to prove,
+but the point is that we don't now have to prove any of them ourselves.
+-/
 end subgroup
 
 end xena
@@ -278,6 +629,7 @@ end xena
 
 /-
 
-Could do bot and top, but would have to practice stuff like mem_singleton
+Further work: `bot` and `top` (would have to explain the
+API for `singleton` and `univ`)
 
 -/
